.

theories/Data/Regex.v
@@ -1,2 +1,41 @@
+Require Import Coq.Lists.List.
 Require Import DschingisKhan.Prelude.PreludeInit.
 Require Import DschingisKhan.Prelude.PreludeMath.
+
+Module RegularExpressions.
+
+  Import ListNotations.
+
+  Section REGULAR_EXPRESSION.
+
+  Context {A : Type}.
+
+  Inductive regex : Type :=
+  | ReZero : regex
+  | ReUnit : regex
+  | ReChar (ch : A) : regex
+  | RePlus (re1 : regex) (re2 : regex) : regex
+  | ReMult (re1 : regex) (re2 : regex) : regex
+  .
+
+  Fixpoint evalRegex (re : regex) {struct re} : ensemble (list A) :=
+    match re with
+    | ReZero => empty
+    | ReUnit => singleton []
+    | ReChar ch => singleton [ch]
+    | RePlus re1 re2 => union (evalRegex re1) (evalRegex re2)
+    | ReMult re1 re2 => liftM2 (@app A) (evalRegex re1) (evalRegex re2)
+    end
+  .
+
+  Global Instance regex_isSetoid : isSetoid regex :=
+    { eqProp (lhs : regex) (rhs : regex) := evalRegex lhs == evalRegex rhs
+    ; eqProp_Equivalence := relation_on_image_liftsEquivalence evalRegex (@eqProp_Equivalence (ensemble (list A)) (ensemble_isSetoid (list A)))
+    }
+  .
+
+  End REGULAR_EXPRESSION.
+
+  Global Arguments regex : clear implicits.
+
+End RegularExpressions.
